Define `map_diff` and prove its termination
In order to prove the termination of the version of Dijkstra that doesn't use
the decreaseKey operation on priority queues, we need to define the difference
operation on balanced maps.
We had to prove a few lemmas about the size of balanced maps when operations are
applied on them to prove the termination of this diff operation.

translator/okasaki-examples/DijkstraScript.sml
@@ -5,12 +5,14 @@
 
 open preamble;
 open SkewBinomialHeapTheory;
+open balanced_mapTheory;
+open mlmapTheory;
+open MapProgTheory;
+open comparisonTheory;
 
 val _ = new_theory "Djikstra";
 
 Datatype `vertex = Vertex 'a (('a # num) list)`;
-
-EVAL ``Vertex #"a" [(#"b", 1); (#"c", 4)]``;
 
 val _ = type_abbrev("graph", ``:'a vertex list``);
 
@@ -131,7 +133,8 @@ val update_distances_def = Define `
           (update_distances dist_without_adj weight adjs)
     in
       if geq_inf old_dist new_dist
-      then ((ElemPrio adj new_dist)::updated_rest, (adj, new_dist)::updated_dists_rest)
+      then ((ElemPrio adj new_dist)::updated_rest,
+	    (adj, new_dist)::updated_dists_rest)
       else (updated_rest, (adj, old_dist)::updated_dists_rest))
 `;
 
@@ -139,32 +142,548 @@ val update_distances_def = Define `
  Djikstra's algorithm itself
 *)
 val dijkstra_step_defn = Hol_defn "dijkstra_step" `
-  dijkstra_step g dists queue =
+  dijkstra_step g dists queue decided =
     if b_is_empty queue
     then dists
     else
       (case (THE (b_find_min queue)) of
        (ElemPrio (label_min:'a) (dist_min: infiNum)) =>
        let queue = THE (b_delete_min geq queue) in
-       let adj_vertices = get_adjacents label_min g in
-       let (updated_vertices, new_distances) =
-         update_distances dists dist_min adj_vertices in
-       dijkstra_step g new_distances
-                     (b_insert_list geq updated_vertices queue))
+       let current_distance = THE (get_distance dists label_min) in
+       if (IS_SOME (lookup decided label_min)) then
+         let adj_vertices = get_adjacents label_min g in
+         let (updated_vertices, new_distances) =
+	      update_distances dists dist_min adj_vertices in
+	   dijkstra_step g
+                         new_distances
+                         (b_insert_list geq updated_vertices queue)
+                         (insert decided label_min T)
+       else
+         dijkstra_step g dists queue decided)
 `;
 
-(* Termination of dijkstra step *)
-Defn.tgoal dijkstra_step_defn;
+(*
+Termination of dijkstra step
+*)
 
+(* size of a map *)
+(* val map_size_def = Define ` *)
+(*   (map_size s = foldrWithKey (\_ _ x. x+1) (0:num) s) *)
+(* `; *)
+
+(* Take one key from the map (not specified which one)*)
+val one_key_def = Define `
+  (one_key Tip = NONE) /\
+  (one_key (Bin _ k v _ _) = SOME k)
+`;
+
+val map_diff_defn = Hol_defn "map_diff" `
+  (map_diff cmp s1 s2 =
+    if (good_cmp cmp) /\ (invariant cmp s1) /\ (invariant cmp s2)
+    then
+      (if (balanced_map$null s2) \/ (balanced_map$null s1)
+       then s1
+       else (let k = THE (one_key s1) in
+         if (IS_SOME (balanced_map$lookup cmp k s2))
+         then map_diff cmp (balanced_map$delete cmp k s1) s2
+         else balanced_map$insert cmp k T
+              (map_diff cmp (balanced_map$delete cmp k s1) s2)))
+    else ARB)
+`;
+
+val map_size_def = Define `
+  (map_size (Map cmp t) = structure_size t)
+`;
+
+Theorem almost_balancedL_aux:
+  !cmp n k v n' k' v' b1 b2.
+    (good_cmp cmp) /\
+    (invariant cmp (Bin n k v Tip (Bin n' k' v' b1 b2))) /\
+    almost_balancedL (size (Bin n k v Tip (Bin n' k' v' b1 b2)))
+                     (size Tip) ==>
+    (b1 = Tip) /\ (b2 = Tip)
+Proof
+  rpt gen_tac \\
+  Cases_on `b1`
+  >- (Cases_on `b2`
+      >- rw[]
+      >- (rw[almost_balancedL_def] \\
+	  (DISJ2_TAC \\ DISJ1_TAC \\
+           disch_tac \\
+           fs[invariant_def, structure_size_def, size_def, balanced_def])))
+  >- (Cases_on `b2` \\
+      (rw[almost_balancedL_def] \\
+	  (DISJ2_TAC \\ DISJ1_TAC \\
+           disch_tac \\
+           fs[invariant_def, structure_size_def, size_def, balanced_def])))
+QED;
+
+Theorem almost_balancedR_aux:
+  !cmp n k v n' k' v' b1 b2.
+    (good_cmp cmp) /\
+    (invariant cmp (Bin n k v (Bin n' k' v' b1 b2) Tip)) /\
+    almost_balancedR (size Tip)
+                     (size (Bin n k v (Bin n' k' v' b1 b2) Tip)) ==>
+    (b1 = Tip) /\ (b2 = Tip)
+Proof
+  rpt gen_tac \\
+  Cases_on `b1`
+  >- (Cases_on `b2`
+      >- rw[]
+      >- (rw[almost_balancedR_def] \\
+          DISJ2_TAC \\ DISJ1_TAC \\
+          disch_tac \\
+          fs[invariant_def, structure_size_def, size_def, balanced_def]))
+  >- (Cases_on `b2` \\
+      (rw[almost_balancedL_def] \\
+	  (DISJ2_TAC \\ DISJ1_TAC \\
+           disch_tac \\
+           fs[invariant_def, structure_size_def, size_def, balanced_def])))
+QED;
+
+Theorem size_bin_lower_bound:
+  !cmp n k v b1 b2. (good_cmp cmp) /\
+                    (invariant cmp (Bin n k v b1 b2)) ==>
+                    size (Bin n k v b1 b2) >= 1
+Proof
+  rw[size_def, invariant_def]
+QED;
+
+Theorem structure_size_thm:
+  !cmp t. invariant cmp t ==> size t = structure_size t
+Proof
+  Cases_on `t` \\
+  rw[invariant_def, size_def, structure_size_def]
+QED;
+
+Theorem balanceL_size:
+  !cmp k v l r. good_cmp cmp /\
+                invariant cmp l /\
+                invariant cmp r /\
+                almost_balancedL (size l) (size r) ==>
+                structure_size (balanceL k v l r) =
+                1 + structure_size l + structure_size r
+Proof
+  Cases_on `l`
+  >- (Cases_on `r`
+      >- rw[balanceL_def, structure_size_def]
+      >- rw[balanceL_def, structure_size_def])
+  >- (Cases_on `r`
+      >- (Cases_on `b`
+          >- (Cases_on `b0`
+              >- rw[balanceL_def, structure_size_def]
+              >- (rw[balanceL_def, structure_size_def] \\
+                 (* We prove that b and b0 must be Tip because l and r
+                    are almost balancedL *)
+                 imp_res_tac almost_balancedL_aux \\
+		 rfs[structure_size_def]))
+          >- (Cases_on `b0`
+              >- rw[balanceL_def, structure_size_def]
+              >- rw[balanceL_def, structure_size_def]))
+      >- (rw[balanceL_def, almost_balancedL_def]
+	  >- (imp_res_tac size_bin_lower_bound \\
+              decide_tac)
+          >- (fs[balanced_def] \\
+              imp_res_tac size_bin_lower_bound
+              >- decide_tac
+	      >- fs[size_def])
+	  >- (imp_res_tac size_bin_lower_bound \\
+              decide_tac)
+	  >- (fs[balanced_def] \\
+              imp_res_tac size_bin_lower_bound
+              >- decide_tac
+              >- fs[size_def, delta_def, structure_size_def])
+          >- (imp_res_tac size_bin_lower_bound \\
+              decide_tac)
+          >- (imp_res_tac size_bin_lower_bound \\
+              decide_tac)
+	  >- (fs[size_def,delta_def] \\
+              Cases_on `b`
+              >- (rw[structure_size_def] \\
+                  fs[invariant_def, structure_size_def, balanced_def,
+		     size_def] \\
+		  imp_res_tac structure_size_thm \\
+                  fs[])
+	      >- (rw[structure_size_def] \\
+                  Cases_on `b0`
+                  >- (rw[structure_size_def] \\
+		      fs[invariant_def, structure_size_def, balanced_def,
+			 size_def])
+                  >- rw[structure_size_def]))
+          >- fs[size_def, delta_def]
+          >- (fs[size_def, delta_def] \\
+              Cases_on `b`
+              >- (rw[structure_size_def] \\
+                  fs[invariant_def, structure_size_def, balanced_def,
+		     size_def] \\
+		  imp_res_tac structure_size_thm \\
+                  fs[])
+              >- (rw[structure_size_def] \\
+                  Cases_on `b0`
+                  >- (rw[structure_size_def] \\
+                      fs[invariant_def, structure_size_def, balanced_def,
+			 size_def])
+                  >- rw[structure_size_def]))
+          >- fs[size_def, delta_def]))
+QED;
+
+Theorem balanceR_size:
+  !cmp k v l r. good_cmp cmp /\
+                invariant cmp l /\
+                invariant cmp r /\
+                almost_balancedR (size l) (size r) ==>
+                structure_size (balanceR k v l r) =
+                1 + structure_size l + structure_size r
+Proof
+  Cases_on `l`
+  >- (Cases_on `r`
+      >- rw[balanceR_def, structure_size_def]
+      >- (Cases_on `b`
+          >- (Cases_on `b0`
+              >- rw[balanceR_def, structure_size_def]
+	      >- rw[balanceR_def, structure_size_def])
+          >- (Cases_on `b0`
+              >- (rw[balanceR_def, structure_size_def] \\
+                  imp_res_tac almost_balancedR_aux \\
+		  rfs[structure_size_def])
+              >- rw[balanceR_def, structure_size_def])))
+  >- (Cases_on `r`
+      >- rw[balanceR_def, structure_size_def]
+      >- (rw[balanceR_def, almost_balancedR_def]
+          >- (imp_res_tac size_bin_lower_bound \\
+              decide_tac)
+	  >- (fs[balanced_def] \\
+              imp_res_tac size_bin_lower_bound
+              >- decide_tac
+	      >- fs[size_def])
+	  >- (imp_res_tac size_bin_lower_bound \\
+              decide_tac)
+	  >- (fs[balanced_def] \\
+              imp_res_tac size_bin_lower_bound
+              >- decide_tac
+              >- fs[size_def, delta_def, structure_size_def])
+          >- (imp_res_tac size_bin_lower_bound \\
+              decide_tac)
+          >- (imp_res_tac size_bin_lower_bound \\
+              decide_tac)
+	  >- (fs[size_def,delta_def] \\
+              Cases_on `b'`
+              >- (rw[structure_size_def] \\
+                  fs[invariant_def, structure_size_def, balanced_def,
+		     size_def] \\
+		  imp_res_tac structure_size_thm \\
+                  fs[])
+	      >- (rw[structure_size_def] \\
+                  Cases_on `b0'`
+                  >- (rw[structure_size_def] \\
+		      fs[invariant_def, structure_size_def, balanced_def,
+			 size_def])
+                  >- rw[structure_size_def]))
+          >- fs[size_def, delta_def]
+          >- (fs[size_def, delta_def] \\
+              Cases_on `b'`
+              >- (rw[structure_size_def] \\
+                  fs[invariant_def, structure_size_def, balanced_def,
+		     size_def] \\
+		  imp_res_tac structure_size_thm \\
+                  fs[])
+              >- (rw[structure_size_def] \\
+                  Cases_on `b0'`
+                  >- (rw[structure_size_def] \\
+                      fs[invariant_def, structure_size_def, balanced_def,
+			 size_def])
+                  >- rw[structure_size_def]))
+          >- fs[size_def, delta_def]))
+QED;
+
+Theorem balanced_is_almostBalancedL:
+  !b1 b2. balanced (size b1) (size b2) ==> almost_balancedL (size b1) (size b2)
+Proof
+  rw[balanced_def, almost_balancedL_def, delta_def, size_def]
+  >- (DISJ2_TAC \\ decide_tac)
+  >- (DISJ2_TAC \\
+      Cases_on `(size b1) < 1`
+      >- fs[]
+      >- fs[MIN_DEF])
+  >- (DISJ1_TAC \\
+      Cases_on `(size b1) < (size b2)` \\
+      fs[MIN_DEF])
+QED;
+
+Theorem balanced_is_almostBalancedR:
+  !b1 b2. balanced (size b1) (size b2) ==> almost_balancedR (size b1) (size b2)
+Proof
+  rw[balanced_def, almost_balancedR_def, delta_def, size_def]
+  >- (DISJ2_TAC \\ decide_tac)
+  >- (DISJ2_TAC \\
+      Cases_on `(size b1) < 1`
+      >- fs[]
+      >- fs[MIN_DEF])
+  >- (DISJ1_TAC \\
+      Cases_on `(size b1) < (size b2)` \\
+      fs[MIN_DEF])
+QED;
+
+
+Theorem balanced_sym:
+  !b1 b2. balanced (size b1) (size b2) ==> balanced (size b2) (size b1)
+Proof
+  rw[balanced_def]
+  >- (DISJ1_TAC \\ decide_tac)
+  >- (DISJ2_TAC \\
+      Cases_on `(size b2) < (size b1)` \\
+      fs[MIN_DEF, delta_def])
+QED;
+
+Theorem deleteFindMax_size:
+  !f km m b l. (good_cmp f) /\
+               ~(balanced_map$null b) /\
+               (invariant f b) /\
+               (deleteFindMax b = ((km,m), l)) ==>
+               structure_size b = (structure_size l) + 1
+Proof
+  ntac 3 strip_tac \\
+  recInduct deleteFindMax_ind \\
+  rpt strip_tac
+  >- fs[deleteFindMax_def, structure_size_def]
+  >- (fs[deleteFindMax_def] \\
+      `~null (Bin v5 v6 v7 v8 v9)` by rw[balanced_mapTheory.null_def] \\
+      `invariant f (Bin v5 v6 v7 v8 v9)` by fs[invariant_def] \\
+      Cases_on `deleteFindMax (Bin v5 v6 v7 v8 v9)` \\
+      Cases_on `q` \\
+      fs[] \\
+      rw[structure_size_def] \\
+      sg `almost_balancedL (size l) (size r)`
+      >- (`invariant f (Bin v5 v6 v7 v8 v9)` by fs[invariant_def] \\
+          `structure_size (Bin v5 v6 v7 v8 v9) = size (Bin v5 v6 v7 v8 v9)`
+          by (imp_res_tac (GSYM structure_size_thm)) \\
+	  `invariant f r` by (imp_res_tac deleteFindMax) \\
+	  `structure_size r = size r`
+          by (imp_res_tac (GSYM structure_size_thm)) \\
+	  fs[size_def] \\
+	  fs[almost_balancedL_def] \\
+          rw[balanced_def, delta_def]
+	  >- (DISJ1_TAC \\ rw[])
+	  >- (fs[invariant_def, balanced_def, size_def, structure_size_def,
+		 delta_def] \\
+              Cases_on `(size l) < (size r + 1)` \\
+              fs[MIN_DEF])
+          >- (fs[invariant_def, balanced_def, size_def] \\
+              Cases_on `(size l) < 1` \\
+              rw[] \\
+	      fs[MIN_DEF, delta_def])
+          >- (fs[invariant_def, balanced_def, size_def, structure_size_def,
+		 delta_def] \\
+              Cases_on `(size l) < 2` \\
+              rw[] \\
+              fs[MIN_DEF])
+	  >- (fs[invariant_def, balanced_def, size_def, structure_size_def,
+		delta_def] \\
+              Cases_on `(size l) < (size r + 1)` \\
+              fs[MIN_DEF, delta_def]))
+      >- (`invariant f l` by fs[invariant_def] \\
+          `invariant f r` by (imp_res_tac deleteFindMax) \\
+	  sg `structure_size (balanceL k x l r) =
+              1 + structure_size l + structure_size r`
+          >- (imp_res_tac balanceL_size \\
+	     first_x_assum (qspecl_then [`x`, `k`] assume_tac) \\
+             rw[])
+	  >- rw[]))
+  >- fs[balanced_mapTheory.null_def]
+QED;
+
+Theorem deleteFindMin_size:
+  !f km m b l. (good_cmp f) /\
+               ~(balanced_map$null b) /\
+               (invariant f b) /\
+               (deleteFindMin b = ((km,m), l)) ==>
+               structure_size b = (structure_size l) + 1
+Proof
+  ntac 3 strip_tac \\
+  recInduct deleteFindMin_ind \\
+  rpt strip_tac
+  >- fs[deleteFindMin_def, structure_size_def]
+  >- (fs[deleteFindMin_def] \\
+      `~null (Bin v5 v6 v7 v8 v9)` by rw[balanced_mapTheory.null_def] \\
+      `invariant f (Bin v5 v6 v7 v8 v9)` by fs[invariant_def] \\
+      Cases_on `deleteFindMin (Bin v5 v6 v7 v8 v9)` \\
+      Cases_on `q` \\
+      fs[] \\
+      rw[structure_size_def] \\
+      sg `almost_balancedR (size r') (size r)`
+      >- (`invariant f (Bin v5 v6 v7 v8 v9)` by fs[invariant_def] \\
+          `structure_size (Bin v5 v6 v7 v8 v9) = size (Bin v5 v6 v7 v8 v9)`
+          by (imp_res_tac (GSYM structure_size_thm)) \\
+	  `invariant f r'` by (imp_res_tac deleteFindMin) \\
+	  `structure_size r' = size r'`
+          by (imp_res_tac (GSYM structure_size_thm)) \\
+	  fs[size_def] \\
+	  fs[almost_balancedR_def] \\
+          rw[balanced_def, delta_def]
+	  >- (DISJ1_TAC \\ rw[])
+	  >- (fs[invariant_def, balanced_def, size_def, structure_size_def,
+		 delta_def] \\
+              Cases_on `(size r') < (size r + 1)` \\
+              fs[MIN_DEF])
+          >- (fs[invariant_def, balanced_def, size_def] \\
+              Cases_on `(size r') < 1` \\
+              rw[] \\
+	      fs[MIN_DEF, delta_def])
+          >- (fs[invariant_def, balanced_def, size_def, structure_size_def,
+		 delta_def] \\
+              Cases_on `(size r') < 2` \\
+              rw[] \\
+              fs[MIN_DEF])
+	  >- (fs[invariant_def, balanced_def, size_def, structure_size_def,
+		delta_def] \\
+              Cases_on `(size r') < (size r + 1)` \\
+              fs[MIN_DEF, delta_def]))
+      >- (`invariant f r` by fs[invariant_def] \\
+          `invariant f r'` by (imp_res_tac deleteFindMin) \\
+	  sg `structure_size (balanceR k x r' r) =
+              1 + structure_size r' + structure_size r`
+          >- (imp_res_tac balanceR_size \\
+	     first_x_assum (qspecl_then [`x`, `k`] assume_tac) \\
+             rw[])
+	  >- rw[]))
+  >- fs[balanced_mapTheory.null_def]
+QED;
+
+Theorem glue_size:
+  !f n k v b1 b2.
+    (good_cmp f) /\
+    (invariant f (Bin n k v b1 b2)) ==>
+    structure_size (glue b1 b2) = structure_size b1 + structure_size b2
+Proof
+  Cases_on `b1`
+  >- rw[glue_def,structure_size_def]
+  >- (Cases_on `b2`
+      >- rw[glue_def,structure_size_def]
+      >- (rw[glue_def]
+	  >- (Cases_on `deleteFindMax (Bin n k v b b0)` \\
+              Cases_on `q` \\
+              rw[] \\
+              `invariant f (Bin n k v b b0)` by fs[invariant_def] \\
+	      `~(null (Bin n k v b b0))` by rw[balanced_mapTheory.null_def] \\
+              imp_res_tac deleteFindMax_size \\
+              rpt (WEAKEN_TAC is_forall) \\
+              `invariant f r` by (imp_res_tac deleteFindMax) \\
+              sg `almost_balancedR (size r) (size (Bin n' k' v' b' b0'))`
+              >- (rw[size_def] \\
+                  `invariant f (Bin n k v b b0)` by fs[invariant_def] \\
+		  `structure_size (Bin n k v b b0) = n`
+                  by (imp_res_tac (GSYM structure_size_thm) \\ rw[size_def]) \\
+		  `structure_size r = size r`
+                  by (imp_res_tac (GSYM structure_size_thm)) \\
+                  fs[size_def] \\
+		  fs[almost_balancedR_def, invariant_def, balanced_def,
+		     delta_def, structure_size_def, size_def] \\
+                  rw[] \\
+		  (Cases_on `(size r) <
+                             (structure_size b' + (structure_size b0' + 1))`
+                   >- fs[]
+		   >- fs[MIN_DEF]))
+	      >- (`invariant f (Bin n' k' v' b' b0')` by fs[invariant_def] \\
+                  sg `structure_size (balanceR q' r' r (Bin n' k' v' b' b0')) =
+                  1+(structure_size r)+(structure_size (Bin n' k' v' b' b0'))`
+                  >- (imp_res_tac balanceR_size \\
+                      first_x_assum (qspecl_then [`r'`, `q'`] assume_tac) \\
+                      rw[])
+		  >- rw[]))
+	  >- (Cases_on `deleteFindMin (Bin n' k' v' b' b0')` \\
+              Cases_on `q` \\
+              rw[] \\
+              `invariant f (Bin n' k' v' b' b0')` by fs[invariant_def] \\
+	      `~(null (Bin n' k' v' b' b0'))` by rw[balanced_mapTheory.null_def] \\
+              imp_res_tac deleteFindMin_size \\
+              rpt (WEAKEN_TAC is_forall) \\
+              `invariant f r` by (imp_res_tac deleteFindMin) \\
+              sg `almost_balancedL (size (Bin n k v b b0)) (size r)`
+              >- (rw[size_def] \\
+                  `invariant f (Bin n k v b b0)` by fs[invariant_def] \\
+		  `structure_size (Bin n k v b b0) = n`
+                  by (imp_res_tac (GSYM structure_size_thm) \\ rw[size_def]) \\
+		  `structure_size r = size r`
+                  by (imp_res_tac (GSYM structure_size_thm)) \\
+                  fs[size_def] \\
+		  fs[almost_balancedL_def, invariant_def, balanced_def,
+		     delta_def, structure_size_def, size_def] \\
+                  rw[] \\
+		  Cases_on `(structure_size b + (structure_size b0 + 1)) <
+                            (size r + 1)` \\
+                  fs[MIN_DEF])
+	      >- (`invariant f (Bin n k v b b0)` by fs[invariant_def] \\
+                  sg `structure_size (balanceL q' r' (Bin n k v b b0) r) =
+                  1+(structure_size r)+(structure_size (Bin n k v b b0))`
+                  >- (imp_res_tac balanceL_size \\
+                      first_x_assum (qspecl_then [`r'`, `q'`] assume_tac) \\
+                      rw[])
+		  >- rw[]))))
+QED;
+
+Theorem delete_one_smaller:
+  !s. (good_cmp f) /\
+      (invariant f b) /\
+      ~(balanced_map$null b) ==>
+      balanced_map$structure_size (balanced_map$delete f (THE (one_key b)) b) <
+      balanced_map$structure_size b
+Proof
+  strip_tac \\
+  rw[structure_size_def] \\
+  Cases_on `b`
+  >- fs[null_def, balanced_mapTheory.null_def]
+  >- (rw[one_key_def, THE_DEF, delete_def,
+	 balanced_mapTheory.delete_def] \\
+      sg `f k k = Equal`
+      >- (imp_res_tac good_cmp_thm \\
+          rpt (first_x_assum (qspecl_then [`k`] assume_tac)) \\
+          rw[])
+      >- (rw[structure_size_def] \\
+          `invariant f b'` by fs[invariant_def] \\
+          `invariant f b0` by fs[invariant_def] \\
+          imp_res_tac glue_size \\
+	  rw[]))
+QED;
+
+val (map_diff_def, map_diff_ind) =
+  Defn.tprove (map_diff_defn,
+    wf_rel_tac `measure (\(cmp,s1,_). structure_size s1)` \\
+    CONJ_TAC \\
+    rpt strip_tac \\
+    imp_res_tac delete_one_smaller \\ rw[])
+;
+
+(* map containing all the the nodes of the graph *)
+val map_nodes_def = Define `
+  (map_nodes [] = (empty num_cmp)) /\
+  (map_nodes ((Vertex l adjs)::vs) =
+    insert (union
+            (map_nodes vs)
+            (mlmap$fromList num_cmp (MAP (\ (l,d).(l,T)) adjs)))
+            l T)
+`;
+
+(* EVAL ``map_nodes  *)
+(*   [(Vertex (1:num) [(2:num, 4); (3, 5)]); (Vertex 2 [(1, 4)])] *)
+(* ``; *)
+
+
+
+(* Defn.tgoal dijkstra_step_defn; *)
 val (dijkstra_step_def, dijkstra_step_ind) =
   Defn.tprove (dijkstra_step_defn,
                cheat)
 ;
 
+
+
+
 val dijkstra_def = Define `
   dijkstra source graph =
-    dijkstra_step graph (initial_distances source graph)
+    dijkstra_step graph
+                  (initial_distances source graph)
                   (b_insert geq (ElemPrio source (Num 0)) Bsbempty)
+                  (empty num_cmp)
 `;
 
 open ml_translatorTheory ml_translatorLib;
